examples/new_stack/NewStack01proof.v
@@ -1,0 +1,374 @@
+Require Import NewStack0 NewStack1 HoareDef SimModSem.
+Require Import Coqlib.
+Require Import Universe.
+Require Import Skeleton.
+Require Import PCM.
+Require Import ModSem Behavior.
+Require Import Relation_Definitions.
+
+(*** TODO: export these in Coqlib or Universe ***)
+Require Import Relation_Operators.
+Require Import RelationPairs.
+From ITree Require Import
+     Events.MapDefault.
+From ExtLib Require Import
+     Core.RelDec
+     Structures.Maps
+     Data.Map.FMapAList.
+Require Import TODOYJ.
+Require Import HTactics Logic IPM.
+Require Import OpenDef.
+Require Import Mem1 MemOpen STB.
+
+Set Implicit Arguments.
+
+Local Open Scope nat_scope.
+
+
+
+Section AUX.
+
+  Context `{Σ: GRA.t}.
+
+  Lemma APCK_start_clo
+        (at_most: Ord.t) (n1: Ord.t)
+        (o: ord)
+        r rg (n0: Ord.t) mr_src0 mp_src0 fr_src0
+        mrs_tgt frs_tgt k_src
+        (wf: (Σ * Any.t) * (Σ * Any.t) -> Prop)
+        (eqr: Σ * Any.t * Σ -> Σ * Any.t * Σ -> Any.t -> Any.t -> Prop)
+        stb itr_tgt
+
+        (ATMOST: (at_most < kappa)%ord)
+        (FUEL: (n1 + 5 < n0)%ord)
+
+        (POST: gpaco6 (_sim_itree wf) (cpn6 (_sim_itree wf)) rg rg _ _ eqr n1
+                       (mr_src0, mp_src0, fr_src0,
+                       (interp_hCallE_tgt stb o (KModSem.transl_itr_tgt (_APCK at_most))) >>= k_src)
+                      ((mrs_tgt, frs_tgt),
+                       itr_tgt))
+    :
+      gpaco6 (_sim_itree wf) (cpn6 (_sim_itree wf)) r rg _ _ eqr n0
+              (mr_src0, mp_src0, fr_src0,
+              (interp_hCallE_tgt stb o (KModSem.transl_itr_tgt APCK)) >>= k_src)
+             ((mrs_tgt, frs_tgt),
+              itr_tgt).
+  Proof.
+    unfold APCK. steps. force_l.
+    exists at_most. ired_l.  _step; [by eauto with ord_step|]. steps; [by eauto with ord_step|].
+    unfold guarantee. ired_both. force_l. esplits; et.
+    ired_both. _step; [by eauto with ord_step|]. steps; [by eauto with ord_step|]. ss.
+    guclo lordC_spec. econs; et. rewrite OrdArith.add_O_r. refl.
+  Qed.
+
+  Lemma APCK_step_clo
+        (fn: gname) (next: Ord.t) (n1: Ord.t)
+
+        (o: ord)
+        r rg (n0: Ord.t) mr_src0 mp_src0 fr_src0
+        mrs_tgt frs_tgt k_src
+        (at_most: Ord.t)
+        (wf: (Σ * Any.t) * (Σ * Any.t) -> Prop)
+        (eqr: Σ * Any.t * Σ -> Σ * Any.t * Σ -> Any.t -> Any.t -> Prop)
+        stb itr_tgt
+
+        (FUEL: (n1 + 11 < n0)%ord)
+        (ftsp: ftspec unit unit)
+        (FIND: alist_find fn stb = Some (KModSem.disclose ftsp))
+        (NEXT: (next < at_most)%ord)
+
+        (POST: gpaco6 (_sim_itree wf) (cpn6 (_sim_itree wf)) rg rg _ _ eqr n1
+                      (mr_src0, mp_src0, fr_src0,
+                       (HoareCall true o (KModSem.disclose ftsp) fn (inl tt));;;
+                                 tau;; tau;; (interp_hCallE_tgt stb o (KModSem.transl_itr_tgt (_APCK next)))
+                                               >>= k_src)
+                      ((mrs_tgt, frs_tgt),
+                       itr_tgt))
+    :
+      gpaco6 (_sim_itree wf) (cpn6 (_sim_itree wf)) r rg _ _ eqr n0
+             (mr_src0, mp_src0, fr_src0, (interp_hCallE_tgt stb o (KModSem.transl_itr_tgt (_APCK at_most)))
+                                           >>= k_src)
+             ((mrs_tgt, frs_tgt),
+              itr_tgt).
+  Proof.
+    rewrite unfold_APCK. steps. force_l. exists false. ired_both.
+    _step; [by eauto with ord_step|].
+    steps; [by eauto with ord_step|].
+    force_l. esplits; et.
+    ired_both; _step; [by eauto with ord_step|].
+    steps; [by eauto with ord_step|].
+    force_l; et.
+    ired_both; _step; [by eauto with ord_step|].
+    steps; [by eauto with ord_step|].
+    force_l. esplits; et.
+    ired_both; _step; [by eauto with ord_step|].
+    steps; [by eauto with ord_step|].
+    rewrite FIND. ired_both. rewrite Any.upcast_downcast. ired_both.
+    guclo lordC_spec. econs; et. { rewrite OrdArith.add_O_r. refl. }
+    match goal with
+    | [SIM: gpaco6 _ _ _ _ _ _ _ _ ?i0 _ |- gpaco6 _ _ _ _ _ _ _ _ ?i1 _] =>
+      replace i1 with i0; auto
+    end.
+    f_equal. grind. ired_both. grind. ired_both. grind.
+  Qed.
+
+  Lemma APCK_stop_clo
+        (n1: Ord.t)
+
+        (o: ord)
+        r rg (n0: Ord.t) mr_src0 mp_src0 fr_src0
+        mrs_tgt frs_tgt k_src
+        (at_most: Ord.t)
+        (wf: (Σ * Any.t) * (Σ * Any.t) -> Prop)
+        (eqr: Σ * Any.t * Σ -> Σ * Any.t * Σ -> Any.t -> Any.t -> Prop)
+        stb itr_tgt
+
+        (FUEL: (n1 + 2 < n0)%ord)
+
+        (POST: gpaco6 (_sim_itree wf) (cpn6 (_sim_itree wf)) rg rg _ _ eqr n1
+                      (mr_src0, mp_src0, fr_src0, k_src ())
+                      ((mrs_tgt, frs_tgt),
+                       itr_tgt))
+    :
+      gpaco6 (_sim_itree wf) (cpn6 (_sim_itree wf)) r rg _ _ eqr n0
+              (mr_src0, mp_src0, fr_src0,
+              (interp_hCallE_tgt stb o (KModSem.transl_itr_tgt (_APCK at_most))) >>= k_src)
+             ((mrs_tgt, frs_tgt),
+              itr_tgt).
+  Proof.
+    rewrite unfold_APCK. steps. force_l. exists true.
+    ired_both; _step; [by eauto with ord_step|].
+    ired_both; _step; [by eauto with ord_step|].
+    steps.
+    guclo lordC_spec. econs; et. { rewrite OrdArith.add_O_r. refl. }
+  Qed.
+
+End AUX.
+
+Ltac kstart _at_most :=
+  eapply (APCK_start_clo) with (at_most := _at_most);
+  [eauto with ord_kappa|
+   (try by (eapply Ord.eq_lt_lt; [(symmetry; eapply OrdArith.add_from_nat)|(eapply OrdArith.lt_from_nat; eapply Nat.lt_add_lt_sub_r; eapply Nat.lt_succ_diag_r)]))|
+  ]
+.
+
+Ltac kstep _fn :=
+  eapply (@APCK_step_clo _ _fn);
+  [(try by (eapply Ord.eq_lt_lt; [(symmetry; eapply OrdArith.add_from_nat)|(eapply OrdArith.lt_from_nat; eapply Nat.lt_add_lt_sub_r; eapply Nat.lt_succ_diag_r)]))|
+   (try by (stb_tac; refl))|
+   (eapply OrdArith.lt_from_nat; eapply Nat.lt_succ_diag_r)|
+  ].
+
+Ltac kcatch :=
+  match goal with
+  | [ |- (gpaco6 (_sim_itree _) _ _ _ _ _ _ _ (_, _) (_, trigger (Call ?fn _) >>= _)) ] =>
+    kstep fn
+  end.
+
+Ltac kstop :=
+  eapply APCK_stop_clo;
+  [(try by (eapply Ord.eq_lt_lt; [(symmetry; eapply OrdArith.add_from_nat)|(eapply OrdArith.lt_from_nat; eapply Nat.lt_add_lt_sub_r; eapply Nat.lt_succ_diag_r)]))|].
+
+
+
+
+Section AUX.
+
+  Context `{Σ: GRA.t}.
+
+  Lemma forall_sep_commute
+        X
+        (P Q: X -> iProp')
+    :
+      (∀ x, P x ** Q x) -∗ (∀ x, P x) ** (∀ x, Q x)
+  .
+  Proof.
+    uipropall. ii. rr in H. uipropall.
+    hexploit (@ClassicalChoice.choice X (Σ * Σ) (fun x '(a, b) => P x a /\ Q x b)).
+    { intro x. spc H. uipropall. des. subst. exists (a, b). et. }
+    i. des.
+    ...?
+  Qed.
+
+  Lemma forall_split
+        X (xcond: X -> bool)
+        (P: X -> iProp')
+    :
+      (∀ x, P x) -∗ (∀ x, ⌜xcond x⌝ -* P x) ** (∀ x, ⌜~xcond x⌝ -* P x)
+  .
+  Proof.
+  Qed.
+
+End AUX.
+
+
+
+
+Section SIMMODSEM.
+
+  Context `{Σ: GRA.t}.
+  Context `{@GRA.inG memRA Σ}.
+
+  Let W: Type := ((Σ * Any.t)) * ((Σ * Any.t)).
+
+  (*** TODO: remove redundancy with Stack1.v ***)
+  Fixpoint is_list (ll: val) (xs: list val): iProp :=
+    match xs with
+    | [] => (⌜ll = Vnullptr⌝: iProp)%I
+    | xhd :: xtl =>
+      (∃ lhd ltl, ⌜ll = Vptr lhd 0⌝ ** (OwnM ((lhd,0%Z) |-> [xhd; ltl]))
+                             ** is_list ltl xtl: iProp)%I
+    end
+  .
+
+  Let wf: W -> Prop :=
+    @mk_wf _ unit
+           (fun _ _stk_mgr0 _ =>
+              (∃ stk_mgr0, (⌜<<CAST: _stk_mgr0 = stk_mgr0↑>>⌝) ∧
+                           (∀ handle stk, (⌜<<ABS: stk_mgr0 handle = Some stk>>⌝) -*
+                                    (∃ hd, OwnM ((handle, 0%Z) |-> [hd]) ** is_list hd (map Vint stk))))%I)
+           (fun _ _ _ => ⌜True⌝%I)
+  .
+
+  (*** TODO: remove redundancy with Mem0OpenProof ***)
+  Definition __hide_mark A (a : A) : A := a.
+  Lemma intro_hide_mark: forall A (a: A), a = __hide_mark a. refl. Qed.
+
+  Ltac hide_k := 
+    match goal with
+    | [ |- (gpaco6 _ _ _ _ _ _ _ _ (_, ?isrc >>= ?ksrc) (_, ?itgt >>= ?ktgt)) ] =>
+      erewrite intro_hide_mark with (a:=ksrc);
+      erewrite intro_hide_mark with (a:=ktgt);
+      let name0 := fresh "__KSRC__" in set (__hide_mark ksrc) as name0; move name0 at top;
+      let name0 := fresh "__KTGT__" in set (__hide_mark ktgt) as name0; move name0 at top
+    end.
+
+  Ltac unhide_k :=
+    do 2 match goal with
+    | [ H := __hide_mark _ |- _ ] => subst H
+    end;
+    rewrite <- ! intro_hide_mark
+  .
+
+  Ltac mRename A B :=
+    match goal with
+    | [H: current_iPropL _ ?iprops |- _ ] =>
+      match iprops with
+      | context[(A, ?x)] => mAssert x with A as B; [iApply A|]
+      end
+    end.
+  Ltac mRefresh := on_current ltac:(fun H => move H at bottom).
+
+  (*** TODO: move to Mem1.v ***)
+  Lemma points_to_disj
+        ptr x0 x1
+    :
+      (OwnM (ptr |-> [x0]) -∗ OwnM (ptr |-> [x1]) -* ⌜False⌝)
+  .
+  Proof.
+    destruct ptr as [blk ofs].
+    iIntros "A B". iCombine "A B" as "A". iOwnWf "A" as WF0.
+    unfold points_to in WF0. rewrite ! unfold_points_to in *. repeat (ur in WF0); ss.
+    specialize (WF0 blk ofs). des_ifs; bsimpl; des; des_sumbool; zsimpl; ss; try lia.
+  Qed.
+
+  Variable global_stb: list (string * fspec).
+  Hypothesis STBINCL: stb_incl (DebugStb ++ StackStb ++ MemStb) global_stb.
+
+  Theorem sim_modsem: ModSemPair.sim (NewStack1.StackSem global_stb) NewStack0.StackSem.
+  Proof.
+    econstructor 1 with (wf:=wf); ss; et; swap 2 3.
+    { econs; ss.
+      - eapply to_semantic; cycle 1. { eapply URA.wf_unit. } iIntros "H". iExists _. iSplit; ss. iIntros; ss.
+      - eapply to_semantic; cycle 1. { eapply URA.wf_unit. } iIntros "H". iPureIntro. ss.
+    }
+    econs; ss.
+    { unfold newF. init. harg. destruct varg_src.
+      { ss. des_ifs; mDesAll; ss. }
+      destruct x; mDesAll; ss. des; subst.
+      unfold new_body, ccall. steps. rewrite Any.upcast_downcast in *; clarify. steps. kstart 1.
+
+      kcatch. { eapply STBINCL. stb_tac; ss. } hcall _ (Some _) _ with "A"; ss; et.
+      { iModIntro. iSplitL; ss; et. iPureIntro. esplits; et. instantiate (1:=1%nat). ss. }
+      { ss. }
+      steps. mDesAll. des; clarify. rewrite Any.upcast_downcast in *. clarify. kstop. steps.
+      rename a3 into handle. force_l. exists handle. steps. rewrite Any.upcast_downcast. steps.
+      rename a2 into stk_mgr0. destruct (stk_mgr0 handle) eqn:T.
+      { mAssertPure False; ss. iSpecialize ("A" $! _ _ T). iDestruct "A" as (x) "[A B]".
+        iApply (points_to_disj with "A A1"); et.
+      }
+      force_l; ss. steps.
+
+      hret _; ss.
+      { iModIntro. iSplitL; ss. iExists _. iSplit; ss. iIntros. des_ifs.
+        - des; clarify. et.
+        - iClear "A1". des; clarify. iSpecialize ("A" $! _ _ H0). et.
+      }
+    }
+    econs; ss.
+    { unfold popF. init. harg. destruct varg_src.
+      { ss. des_ifs; mDesAll; ss. }
+      destruct x; mDesAll; ss. des; subst.
+      unfold pop_body, ccall. steps. rewrite Any.upcast_downcast in *; clarify. steps. kstart 7.
+
+      hide_k. destruct v; ss. des_ifs.
+      rename n into handle. rename a0 into stk_mgr0. rename l into stk. rename _UNWRAPU0 into T.
+      mAssert _ with "".
+      { Ltac mRamify A P B :=
+          match goal with
+          | [H: current_iPropL _ ?iprops |- _ ] =>
+            match iprops with
+            | context[(A, ?x)] => mAssert (P ** (P -* x)) with A as B
+            end
+          end.
+        mRamify "A" (((∃ hd : val, OwnM ((handle, 0%Z) |-> [hd]) ** is_list hd (map Vint stk)))%I) "B".
+        {
+
+        match goal with
+        instantiate (1:=((∀ (handle : nat) (stk : list Z),
+             ⌜<<ABS: stk_mgr0 handle = Some stk >>⌝ -*
+             (∃ hd : val, OwnM ((handle, 0%Z) |-> [hd]) ** is_list hd (map Vint stk)))%I)).
+
+      mSpcUniv "A" with handle. mSpcUniv "A" with stk.
+      mAssert _ with "". { instantiate (1:=(⌜_⌝%I)). iPureIntro. exact T. } mSpcWand "A" with "A1".
+      mDesAll. rename a0 into hd. unhide_k.
+
+      kcatch. { eapply STBINCL. stb_tac; ss. } hcall _ (Some _) _ with "A"; ss; et.
+      { iModIntro. iSplitL; ss; et. iPureIntro. esplits; et. instantiate (1:=1%nat). ss. }
+      { ss. }
+      steps. mDesAll. des; clarify. rewrite Any.upcast_downcast in *. clarify. kstop. steps.
+      rename a3 into handle. force_l. exists handle. steps. rewrite Any.upcast_downcast. steps.
+      rename a2 into stk_mgr0. destruct (stk_mgr0 handle) eqn:T.
+      { mAssertPure False; ss. iSpecialize ("A" $! _ _ T). iDestruct "A" as (x) "[A B]".
+        iApply (points_to_disj with "A A1"); et.
+      }
+      force_l; ss. steps.
+
+      hret _; ss.
+      { iModIntro. iSplitL; ss. iExists _. iSplit; ss. iIntros. des_ifs.
+        - des; clarify. et.
+        - iClear "A1". des; clarify. iSpecialize ("A" $! _ _ H0). et.
+      }
+    }
+  Unshelve.
+    all: ss.
+  Qed.
+
+End SIMMODSEM.
+
+
+
+Section SIMMOD.
+
+  Context `{Σ: GRA.t}.
+  Context `{@GRA.inG memRA Σ}.
+
+  Theorem correct: ModPair.sim (MemClient1.Client (fun _ => (UnknownStb ++ ClientStb ++ MemStb)))
+                               MemClient0.Client.
+  Proof.
+    econs; ss.
+    { ii. eapply adequacy_lift. eapply sim_modsem. }
+    ii; ss. repeat (econs; ss).
+  Qed.
+
+End SIMMOD.
